Steel.Effect.Atomic with one assume

pulse/ulib/experimental/Steel.Effect.Atomic.fst
@@ -141,18 +141,27 @@ let atomic_preserves_frame_and_preorder
 #pop-options
 
 #push-options "--fuel 0 --ifuel 0 --z3rlimit 10"
-let frame0 (#a:Type) (#uses:Set.set lock_addr) (#is_ghost:bool) (#pre:pre_t) (#post:post_t a)
-  (f:atomic_repr a uses is_ghost pre post)
-  (frame:hprop)
-: SteelAtomic a
-  uses
-  is_ghost
-  (pre `star` frame)
-  (fun x -> post x `star` frame)
-= SteelAtomic?.reflect (fun _ -> Sem.run #(state_uses uses) #_ #_ #_ #_ #_ (Sem.Frame (Sem.Act f) frame (fun _ -> True)))
+// let frame0 (#a:Type) (#uses:Set.set lock_addr) (#is_ghost:bool) (#pre:pre_t) (#post:post_t a)
+//   (f:atomic_repr a uses is_ghost pre post)
+//   (frame:hprop)
+// : SteelAtomic a
+//   uses
+//   is_ghost
+//   (pre `star` frame)
+//   (fun x -> post x `star` frame)
+// = admit ()
+
+// SteelAtomic?.reflect (fun _ ->
+//     //let m0 = NMSTTotal.get () in
+//     let x = f () in
+//     x)
+
+
+
+// Sem.run #(state_uses uses) #_ #_ #_ #_ #_ (Sem.Frame (Sem.Act f) frame (fun _ -> True)))
 #pop-options
 
-let atomic_frame (#a:Type) (#uses:Set.set lock_addr) (#is_ghost:bool) (#pre:pre_t) (#post:post_t a)
+assume val  atomic_frame (#a:Type) (#uses:Set.set lock_addr) (#is_ghost:bool) (#pre:pre_t) (#post:post_t a)
   (frame:hprop)
   ($f:unit -> SteelAtomic a uses is_ghost pre post)
 : SteelAtomic a
@@ -160,10 +169,10 @@ let atomic_frame (#a:Type) (#uses:Set.set lock_addr) (#is_ghost:bool) (#pre:pre_
   is_ghost
   (pre `star` frame)
   (fun x -> post x `star` frame)
-= frame0 (reify (f ())) frame
+// = admit () //frame0 (reify (f ())) frame
 
 let inv_witnessed (#p:hprop) (i:inv p) =
-  NMST.witnessed mem mem_evolves (inv_ok i)
+  NMSTTotal.witnessed mem mem_evolves (inv_ok i)
 
 let ival (p:hprop) = i:inv p{inv_witnessed i}
 
@@ -176,7 +185,7 @@ let new_inv (p:hprop) : SteelAtomic (ival p) Set.empty false p (fun _ -> emp)
       Classical.forall_intro (Classical.move_requires (new_inv_preserves_frame p m0));
       mst_put m1;
       Classical.forall_intro_2 (inv_ok_stable i);
-      NMST.witness mem mem_evolves (inv_ok i);
+      NMSTTotal.witness mem mem_evolves (inv_ok i);
       i)
 #pop-options
 
@@ -309,13 +318,13 @@ let with_invariant_aux
   (f:atomic_repr a (Set.union (Set.singleton i) uses) is_ghost (p `star` fp) (fun x -> p `star` fp' x))
   : atomic_repr a uses is_ghost fp fp'
   = fun _ ->
-      NMST.recall mem mem_evolves (inv_ok i);
-      let m0 = NMST.get() in
+      NMSTTotal.recall mem mem_evolves (inv_ok i);
+      let m0 = NMSTTotal.get() in
       let s = Set.union (Set.singleton i) uses in
       interp_inv_unused i uses fp m0;
       let x = f () in
-      let m1 = NMST.get() in
-      NMST.recall mem mem_evolves (inv_ok i);
+      let m1 = NMSTTotal.get() in
+      NMSTTotal.recall mem mem_evolves (inv_ok i);
       interp_inv_unused i uses (fp' x) m1;
       lemma_sem_preserves fp (fp' x) m0 m1 uses i;
       x
